instructions/binary_search/a44.v
@@ -1,31 +1,31 @@
 From isla Require Import opsem.
 
 Definition a44 : isla_trace :=
-  Smt (DeclareConst 27%Z (Ty_BitVec 1%N)) Mk_annot :t:
-  Smt (DeclareConst 37%Z (Ty_BitVec 64%N)) Mk_annot :t:
-  ReadReg "R20" [] (RegVal_Base (Val_Symbolic 37%Z)) Mk_annot :t:
-  Smt (DefineConst 38%Z (Val (Val_Symbolic 37%Z) Mk_annot)) Mk_annot :t:
-  Smt (DeclareConst 39%Z (Ty_BitVec 64%N)) Mk_annot :t:
-  ReadReg "R24" [] (RegVal_Base (Val_Symbolic 39%Z)) Mk_annot :t:
-  Smt (DefineConst 40%Z (Val (Val_Symbolic 39%Z) Mk_annot)) Mk_annot :t:
-  ReadReg "PSTATE" [Field "Z"] (RegVal_Struct [("Z", RegVal_Base (Val_Symbolic 27%Z))]) Mk_annot :t:
-  Smt (DefineConst 43%Z (Unop (Not) (Binop (Eq) (Val (Val_Symbolic 27%Z) Mk_annot) (Val (Val_Bits (BV 1%N 0x1%Z)) Mk_annot) Mk_annot) Mk_annot)) Mk_annot :t:
+  Smt (DeclareConst 24%Z (Ty_BitVec 1%N)) Mk_annot :t:
+  Smt (DeclareConst 27%Z (Ty_BitVec 64%N)) Mk_annot :t:
+  ReadReg "R20" [] (RegVal_Base (Val_Symbolic 27%Z)) Mk_annot :t:
+  Smt (DefineConst 28%Z (Val (Val_Symbolic 27%Z) Mk_annot)) Mk_annot :t:
+  Smt (DeclareConst 29%Z (Ty_BitVec 64%N)) Mk_annot :t:
+  ReadReg "R24" [] (RegVal_Base (Val_Symbolic 29%Z)) Mk_annot :t:
+  Smt (DefineConst 30%Z (Val (Val_Symbolic 29%Z) Mk_annot)) Mk_annot :t:
+  ReadReg "PSTATE" [Field "Z"] (RegVal_Struct [("Z", RegVal_Base (Val_Symbolic 24%Z))]) Mk_annot :t:
+  Smt (DefineConst 33%Z (Unop (Not) (Binop (Eq) (Val (Val_Symbolic 24%Z) Mk_annot) (Val (Val_Bits (BV 1%N 0x1%Z)) Mk_annot) Mk_annot) Mk_annot)) Mk_annot :t:
   tcases [
-    Smt (Assert (Val (Val_Symbolic 43%Z) Mk_annot)) Mk_annot :t:
-    Smt (DefineConst 44%Z (Val (Val_Symbolic 38%Z) Mk_annot)) Mk_annot :t:
-    WriteReg "R20" [] (RegVal_Base (Val_Symbolic 44%Z)) Mk_annot :t:
-    Smt (DeclareConst 45%Z (Ty_BitVec 64%N)) Mk_annot :t:
-    ReadReg "_PC" [] (RegVal_Base (Val_Symbolic 45%Z)) Mk_annot :t:
-    Smt (DefineConst 46%Z (Manyop (Bvmanyarith Bvadd) [Val (Val_Symbolic 45%Z) Mk_annot; Val (Val_Bits (BV 64%N 0x4%Z)) Mk_annot] Mk_annot)) Mk_annot :t:
-    WriteReg "_PC" [] (RegVal_Base (Val_Symbolic 46%Z)) Mk_annot :t:
+    Smt (Assert (Val (Val_Symbolic 33%Z) Mk_annot)) Mk_annot :t:
+    Smt (DefineConst 34%Z (Val (Val_Symbolic 28%Z) Mk_annot)) Mk_annot :t:
+    WriteReg "R20" [] (RegVal_Base (Val_Symbolic 34%Z)) Mk_annot :t:
+    Smt (DeclareConst 35%Z (Ty_BitVec 64%N)) Mk_annot :t:
+    ReadReg "_PC" [] (RegVal_Base (Val_Symbolic 35%Z)) Mk_annot :t:
+    Smt (DefineConst 36%Z (Manyop (Bvmanyarith Bvadd) [Val (Val_Symbolic 35%Z) Mk_annot; Val (Val_Bits (BV 64%N 0x4%Z)) Mk_annot] Mk_annot)) Mk_annot :t:
+    WriteReg "_PC" [] (RegVal_Base (Val_Symbolic 36%Z)) Mk_annot :t:
     tnil;
-    Smt (Assert (Unop (Not) (Val (Val_Symbolic 43%Z) Mk_annot) Mk_annot)) Mk_annot :t:
-    Smt (DefineConst 44%Z (Val (Val_Symbolic 40%Z) Mk_annot)) Mk_annot :t:
-    WriteReg "R20" [] (RegVal_Base (Val_Symbolic 44%Z)) Mk_annot :t:
-    Smt (DeclareConst 45%Z (Ty_BitVec 64%N)) Mk_annot :t:
-    ReadReg "_PC" [] (RegVal_Base (Val_Symbolic 45%Z)) Mk_annot :t:
-    Smt (DefineConst 46%Z (Manyop (Bvmanyarith Bvadd) [Val (Val_Symbolic 45%Z) Mk_annot; Val (Val_Bits (BV 64%N 0x4%Z)) Mk_annot] Mk_annot)) Mk_annot :t:
-    WriteReg "_PC" [] (RegVal_Base (Val_Symbolic 46%Z)) Mk_annot :t:
+    Smt (Assert (Unop (Not) (Val (Val_Symbolic 33%Z) Mk_annot) Mk_annot)) Mk_annot :t:
+    Smt (DefineConst 37%Z (Val (Val_Symbolic 30%Z) Mk_annot)) Mk_annot :t:
+    WriteReg "R20" [] (RegVal_Base (Val_Symbolic 37%Z)) Mk_annot :t:
+    Smt (DeclareConst 38%Z (Ty_BitVec 64%N)) Mk_annot :t:
+    ReadReg "_PC" [] (RegVal_Base (Val_Symbolic 38%Z)) Mk_annot :t:
+    Smt (DefineConst 39%Z (Manyop (Bvmanyarith Bvadd) [Val (Val_Symbolic 38%Z) Mk_annot; Val (Val_Bits (BV 64%N 0x4%Z)) Mk_annot] Mk_annot)) Mk_annot :t:
+    WriteReg "_PC" [] (RegVal_Base (Val_Symbolic 39%Z)) Mk_annot :t:
     tnil
   ]
 .
