instructions/binary_search/a64.v
@@ -10,36 +10,39 @@ Definition a64 : isla_trace :=
   AssumeReg "EDSCR" [] (RegVal_Base (Val_Bits (BV 32%N 0x0%Z))) Mk_annot :t:
   AssumeReg "OSDLR_EL1" [] (RegVal_Base (Val_Bits (BV 32%N 0x0%Z))) Mk_annot :t:
   AssumeReg "OSLSR_EL1" [] (RegVal_Base (Val_Bits (BV 32%N 0x0%Z))) Mk_annot :t:
-  Smt (DeclareConst 6%Z (Ty_BitVec 1%N)) Mk_annot :t:
+  Smt (DeclareConst 3%Z (Ty_BitVec 1%N)) Mk_annot :t:
   AssumeReg "PSTATE" [Field "EL"] (RegVal_Base (Val_Bits (BV 2%N 0x2%Z))) Mk_annot :t:
   AssumeReg "PSTATE" [Field "SP"] (RegVal_Base (Val_Bits (BV 1%N 0x1%Z))) Mk_annot :t:
   AssumeReg "PSTATE" [Field "nRW"] (RegVal_Base (Val_Bits (BV 1%N 0x0%Z))) Mk_annot :t:
   AssumeReg "SCR_EL3" [] (RegVal_Base (Val_Bits (BV 32%N 0x501%Z))) Mk_annot :t:
   AssumeReg "SCTLR_EL2" [] (RegVal_Base (Val_Bits (BV 64%N 0x4000002%Z))) Mk_annot :t:
-  Smt (DeclareConst 29%Z (Ty_BitVec 64%N)) Mk_annot :t:
+  Smt (DeclareConst 26%Z (Ty_BitVec 64%N)) Mk_annot :t:
   Assume (AExp_Binop (Eq) (AExp_Manyop (Bvmanyarith Bvand) [AExp_Val (AVal_Var "SP_EL2" []) Mk_annot; AExp_Val (AVal_Bits (BV 64%N 0xfff0000000000007%Z)) Mk_annot] Mk_annot) (AExp_Val (AVal_Bits (BV 64%N 0x0%Z)) Mk_annot) Mk_annot) Mk_annot :t:
   Assume (AExp_Binop (Eq) (AExp_Manyop (Bvmanyarith Bvand) [AExp_Manyop (Bvmanyarith Bvadd) [AExp_Val (AVal_Var "SP_EL2" []) Mk_annot; AExp_Val (AVal_Bits (BV 64%N 0x28%Z)) Mk_annot] Mk_annot; AExp_Val (AVal_Bits (BV 64%N 0xfff0000000000007%Z)) Mk_annot] Mk_annot) (AExp_Val (AVal_Bits (BV 64%N 0x0%Z)) Mk_annot) Mk_annot) Mk_annot :t:
-  ReadReg "SP_EL2" [] (RegVal_Base (Val_Symbolic 29%Z)) Mk_annot :t:
-  Smt (DefineConst 73%Z (Manyop (Bvmanyarith Bvadd) [Val (Val_Symbolic 29%Z) Mk_annot; Val (Val_Bits (BV 64%N 0x20%Z)) Mk_annot] Mk_annot)) Mk_annot :t:
-  Smt (DefineConst 74%Z (Manyop (Bvmanyarith Bvadd) [Val (Val_Symbolic 73%Z) Mk_annot; Val (Val_Bits (BV 64%N 0x0%Z)) Mk_annot] Mk_annot)) Mk_annot :t:
-  Smt (DefineConst 78%Z (Binop (Eq) (Val (Val_Symbolic 74%Z) Mk_annot) (Manyop (Bvmanyarith Bvand) [Val (Val_Symbolic 74%Z) Mk_annot; Val (Val_Bits (BV 64%N 0xfffffffffffffff8%Z)) Mk_annot] Mk_annot) Mk_annot)) Mk_annot :t:
-  ReadReg "PSTATE" [Field "D"] (RegVal_Struct [("D", RegVal_Base (Val_Symbolic 6%Z))]) Mk_annot :t:
-  Smt (DeclareConst 2289%Z (Ty_BitVec 56%N)) Mk_annot :t:
-  Smt (DefineConst 2298%Z (Unop (ZeroExtend 8%N) (Manyop Concat [Val (Val_Bits (BV 4%N 0x0%Z)) Mk_annot; Unop (Extract 51%N 0%N) (Val (Val_Symbolic 74%Z) Mk_annot) Mk_annot] Mk_annot) Mk_annot)) Mk_annot :t:
-  Smt (DeclareConst 2299%Z (Ty_BitVec 64%N)) Mk_annot :t:
-  ReadMem (RegVal_Base (Val_Symbolic 2299%Z)) (RegVal_Base (Val_Enum ((Mk_enum_id 6%nat), Mk_enum_ctor 0%nat))) (RegVal_Base (Val_Symbolic 2298%Z)) 8%N None Mk_annot :t:
-  Smt (DefineConst 2302%Z (Manyop (Bvmanyarith Bvadd) [Val (Val_Symbolic 73%Z) Mk_annot; Val (Val_Bits (BV 64%N 0x8%Z)) Mk_annot] Mk_annot)) Mk_annot :t:
-  Smt (DefineConst 2306%Z (Binop (Eq) (Val (Val_Symbolic 2302%Z) Mk_annot) (Manyop (Bvmanyarith Bvand) [Val (Val_Symbolic 2302%Z) Mk_annot; Val (Val_Bits (BV 64%N 0xfffffffffffffff8%Z)) Mk_annot] Mk_annot) Mk_annot)) Mk_annot :t:
-  Smt (DefineConst 4496%Z (Unop (ZeroExtend 8%N) (Manyop Concat [Val (Val_Bits (BV 4%N 0x0%Z)) Mk_annot; Unop (Extract 51%N 0%N) (Val (Val_Symbolic 2302%Z) Mk_annot) Mk_annot] Mk_annot) Mk_annot)) Mk_annot :t:
-  Smt (DeclareConst 4497%Z (Ty_BitVec 64%N)) Mk_annot :t:
-  ReadMem (RegVal_Base (Val_Symbolic 4497%Z)) (RegVal_Base (Val_Enum ((Mk_enum_id 6%nat), Mk_enum_ctor 0%nat))) (RegVal_Base (Val_Symbolic 4496%Z)) 8%N None Mk_annot :t:
-  Smt (DefineConst 4500%Z (Val (Val_Symbolic 2299%Z) Mk_annot)) Mk_annot :t:
-  WriteReg "R22" [] (RegVal_Base (Val_Symbolic 4500%Z)) Mk_annot :t:
-  Smt (DefineConst 4501%Z (Val (Val_Symbolic 4497%Z) Mk_annot)) Mk_annot :t:
-  WriteReg "R21" [] (RegVal_Base (Val_Symbolic 4501%Z)) Mk_annot :t:
-  Smt (DeclareConst 4502%Z (Ty_BitVec 64%N)) Mk_annot :t:
-  ReadReg "_PC" [] (RegVal_Base (Val_Symbolic 4502%Z)) Mk_annot :t:
-  Smt (DefineConst 4503%Z (Manyop (Bvmanyarith Bvadd) [Val (Val_Symbolic 4502%Z) Mk_annot; Val (Val_Bits (BV 64%N 0x4%Z)) Mk_annot] Mk_annot)) Mk_annot :t:
-  WriteReg "_PC" [] (RegVal_Base (Val_Symbolic 4503%Z)) Mk_annot :t:
+  ReadReg "SP_EL2" [] (RegVal_Base (Val_Symbolic 26%Z)) Mk_annot :t:
+  Smt (DefineConst 36%Z (Manyop (Bvmanyarith Bvadd) [Val (Val_Symbolic 26%Z) Mk_annot; Val (Val_Bits (BV 64%N 0x20%Z)) Mk_annot] Mk_annot)) Mk_annot :t:
+  Smt (DefineConst 37%Z (Manyop (Bvmanyarith Bvadd) [Val (Val_Symbolic 36%Z) Mk_annot; Val (Val_Bits (BV 64%N 0x0%Z)) Mk_annot] Mk_annot)) Mk_annot :t:
+  Smt (DefineConst 41%Z (Binop (Eq) (Val (Val_Symbolic 37%Z) Mk_annot) (Manyop (Bvmanyarith Bvand) [Val (Val_Symbolic 37%Z) Mk_annot; Val (Val_Bits (BV 64%N 0xfffffffffffffff8%Z)) Mk_annot] Mk_annot) Mk_annot)) Mk_annot :t:
+  ReadReg "PSTATE" [Field "D"] (RegVal_Struct [("D", RegVal_Base (Val_Symbolic 3%Z))]) Mk_annot :t:
+  Smt (DefineConst 1216%Z (Val (Val_Symbolic 37%Z) Mk_annot)) Mk_annot :t:
+  Smt (DefineConst 1364%Z (Manyop Concat [Val (Val_Bits (BV 4%N 0x0%Z)) Mk_annot; Unop (Extract 51%N 0%N) (Val (Val_Symbolic 37%Z) Mk_annot) Mk_annot] Mk_annot)) Mk_annot :t:
+  Smt (DefineConst 1365%Z (Unop (ZeroExtend 8%N) (Val (Val_Symbolic 1364%Z) Mk_annot) Mk_annot)) Mk_annot :t:
+  Smt (DeclareConst 1366%Z (Ty_BitVec 64%N)) Mk_annot :t:
+  ReadMem (RegVal_Base (Val_Symbolic 1366%Z)) (RegVal_Poison) (RegVal_Base (Val_Symbolic 1365%Z)) 8%N None Mk_annot :t:
+  Smt (DefineConst 1369%Z (Manyop (Bvmanyarith Bvadd) [Val (Val_Symbolic 36%Z) Mk_annot; Val (Val_Bits (BV 64%N 0x8%Z)) Mk_annot] Mk_annot)) Mk_annot :t:
+  Smt (DefineConst 1373%Z (Binop (Eq) (Val (Val_Symbolic 1369%Z) Mk_annot) (Manyop (Bvmanyarith Bvand) [Val (Val_Symbolic 1369%Z) Mk_annot; Val (Val_Bits (BV 64%N 0xfffffffffffffff8%Z)) Mk_annot] Mk_annot) Mk_annot)) Mk_annot :t:
+  Smt (DefineConst 2548%Z (Val (Val_Symbolic 1369%Z) Mk_annot)) Mk_annot :t:
+  Smt (DefineConst 2696%Z (Manyop Concat [Val (Val_Bits (BV 4%N 0x0%Z)) Mk_annot; Unop (Extract 51%N 0%N) (Val (Val_Symbolic 1369%Z) Mk_annot) Mk_annot] Mk_annot)) Mk_annot :t:
+  Smt (DefineConst 2697%Z (Unop (ZeroExtend 8%N) (Val (Val_Symbolic 2696%Z) Mk_annot) Mk_annot)) Mk_annot :t:
+  Smt (DeclareConst 2698%Z (Ty_BitVec 64%N)) Mk_annot :t:
+  ReadMem (RegVal_Base (Val_Symbolic 2698%Z)) (RegVal_Poison) (RegVal_Base (Val_Symbolic 2697%Z)) 8%N None Mk_annot :t:
+  Smt (DefineConst 2701%Z (Val (Val_Symbolic 1366%Z) Mk_annot)) Mk_annot :t:
+  WriteReg "R22" [] (RegVal_Base (Val_Symbolic 2701%Z)) Mk_annot :t:
+  Smt (DefineConst 2702%Z (Val (Val_Symbolic 2698%Z) Mk_annot)) Mk_annot :t:
+  WriteReg "R21" [] (RegVal_Base (Val_Symbolic 2702%Z)) Mk_annot :t:
+  Smt (DeclareConst 2703%Z (Ty_BitVec 64%N)) Mk_annot :t:
+  ReadReg "_PC" [] (RegVal_Base (Val_Symbolic 2703%Z)) Mk_annot :t:
+  Smt (DefineConst 2704%Z (Manyop (Bvmanyarith Bvadd) [Val (Val_Symbolic 2703%Z) Mk_annot; Val (Val_Bits (BV 64%N 0x4%Z)) Mk_annot] Mk_annot)) Mk_annot :t:
+  WriteReg "_PC" [] (RegVal_Base (Val_Symbolic 2704%Z)) Mk_annot :t:
   tnil
 .
