instructions/binary_search/ac.v
@@ -10,40 +10,43 @@ Definition ac : isla_trace :=
   AssumeReg "EDSCR" [] (RegVal_Base (Val_Bits (BV 32%N 0x0%Z))) Mk_annot :t:
   AssumeReg "OSDLR_EL1" [] (RegVal_Base (Val_Bits (BV 32%N 0x0%Z))) Mk_annot :t:
   AssumeReg "OSLSR_EL1" [] (RegVal_Base (Val_Bits (BV 32%N 0x0%Z))) Mk_annot :t:
-  Smt (DeclareConst 6%Z (Ty_BitVec 1%N)) Mk_annot :t:
+  Smt (DeclareConst 3%Z (Ty_BitVec 1%N)) Mk_annot :t:
   AssumeReg "PSTATE" [Field "EL"] (RegVal_Base (Val_Bits (BV 2%N 0x2%Z))) Mk_annot :t:
   AssumeReg "PSTATE" [Field "SP"] (RegVal_Base (Val_Bits (BV 1%N 0x1%Z))) Mk_annot :t:
   AssumeReg "PSTATE" [Field "nRW"] (RegVal_Base (Val_Bits (BV 1%N 0x0%Z))) Mk_annot :t:
   AssumeReg "SCR_EL3" [] (RegVal_Base (Val_Bits (BV 32%N 0x501%Z))) Mk_annot :t:
   AssumeReg "SCTLR_EL2" [] (RegVal_Base (Val_Bits (BV 64%N 0x4000002%Z))) Mk_annot :t:
-  Smt (DeclareConst 29%Z (Ty_BitVec 64%N)) Mk_annot :t:
+  Smt (DeclareConst 26%Z (Ty_BitVec 64%N)) Mk_annot :t:
   Assume (AExp_Binop (Eq) (AExp_Manyop (Bvmanyarith Bvand) [AExp_Val (AVal_Var "SP_EL2" []) Mk_annot; AExp_Val (AVal_Bits (BV 64%N 0xfff0000000000007%Z)) Mk_annot] Mk_annot) (AExp_Val (AVal_Bits (BV 64%N 0x0%Z)) Mk_annot) Mk_annot) Mk_annot :t:
   Assume (AExp_Binop (Eq) (AExp_Manyop (Bvmanyarith Bvand) [AExp_Manyop (Bvmanyarith Bvadd) [AExp_Val (AVal_Var "SP_EL2" []) Mk_annot; AExp_Val (AVal_Bits (BV 64%N 0x38%Z)) Mk_annot] Mk_annot; AExp_Val (AVal_Bits (BV 64%N 0xfff0000000000007%Z)) Mk_annot] Mk_annot) (AExp_Val (AVal_Bits (BV 64%N 0x0%Z)) Mk_annot) Mk_annot) Mk_annot :t:
-  ReadReg "SP_EL2" [] (RegVal_Base (Val_Symbolic 29%Z)) Mk_annot :t:
-  Smt (DefineConst 73%Z (Manyop (Bvmanyarith Bvadd) [Val (Val_Symbolic 29%Z) Mk_annot; Val (Val_Bits (BV 64%N 0x30%Z)) Mk_annot] Mk_annot)) Mk_annot :t:
-  Smt (DeclareConst 74%Z (Ty_BitVec 64%N)) Mk_annot :t:
-  ReadReg "R20" [] (RegVal_Base (Val_Symbolic 74%Z)) Mk_annot :t:
-  Smt (DefineConst 75%Z (Val (Val_Symbolic 74%Z) Mk_annot)) Mk_annot :t:
-  Smt (DeclareConst 76%Z (Ty_BitVec 64%N)) Mk_annot :t:
-  ReadReg "R19" [] (RegVal_Base (Val_Symbolic 76%Z)) Mk_annot :t:
-  Smt (DefineConst 77%Z (Val (Val_Symbolic 76%Z) Mk_annot)) Mk_annot :t:
-  Smt (DefineConst 78%Z (Manyop (Bvmanyarith Bvadd) [Val (Val_Symbolic 73%Z) Mk_annot; Val (Val_Bits (BV 64%N 0x0%Z)) Mk_annot] Mk_annot)) Mk_annot :t:
-  Smt (DefineConst 83%Z (Binop (Eq) (Val (Val_Symbolic 78%Z) Mk_annot) (Manyop (Bvmanyarith Bvand) [Val (Val_Symbolic 78%Z) Mk_annot; Val (Val_Bits (BV 64%N 0xfffffffffffffff8%Z)) Mk_annot] Mk_annot) Mk_annot)) Mk_annot :t:
-  ReadReg "PSTATE" [Field "D"] (RegVal_Struct [("D", RegVal_Base (Val_Symbolic 6%Z))]) Mk_annot :t:
-  Smt (DeclareConst 2117%Z (Ty_BitVec 64%N)) Mk_annot :t:
-  ReadReg "MPIDR_EL1" [] (RegVal_Base (Val_Symbolic 2117%Z)) Mk_annot :t:
-  Smt (DeclareConst 2300%Z (Ty_BitVec 56%N)) Mk_annot :t:
-  Smt (DefineConst 2313%Z (Unop (ZeroExtend 8%N) (Manyop Concat [Val (Val_Bits (BV 4%N 0x0%Z)) Mk_annot; Unop (Extract 51%N 0%N) (Val (Val_Symbolic 78%Z) Mk_annot) Mk_annot] Mk_annot) Mk_annot)) Mk_annot :t:
-  Smt (DeclareConst 2314%Z Ty_Bool) Mk_annot :t:
-  WriteMem (RegVal_Base (Val_Symbolic 2314%Z)) (RegVal_Base (Val_Enum ((Mk_enum_id 6%nat), Mk_enum_ctor 0%nat))) (RegVal_Base (Val_Symbolic 2313%Z)) (RegVal_Base (Val_Symbolic 75%Z)) 8%N None Mk_annot :t:
-  Smt (DefineConst 2315%Z (Manyop (Bvmanyarith Bvadd) [Val (Val_Symbolic 73%Z) Mk_annot; Val (Val_Bits (BV 64%N 0x8%Z)) Mk_annot] Mk_annot)) Mk_annot :t:
-  Smt (DefineConst 2320%Z (Binop (Eq) (Val (Val_Symbolic 2315%Z) Mk_annot) (Manyop (Bvmanyarith Bvand) [Val (Val_Symbolic 2315%Z) Mk_annot; Val (Val_Bits (BV 64%N 0xfffffffffffffff8%Z)) Mk_annot] Mk_annot) Mk_annot)) Mk_annot :t:
-  Smt (DefineConst 4515%Z (Unop (ZeroExtend 8%N) (Manyop Concat [Val (Val_Bits (BV 4%N 0x0%Z)) Mk_annot; Unop (Extract 51%N 0%N) (Val (Val_Symbolic 2315%Z) Mk_annot) Mk_annot] Mk_annot) Mk_annot)) Mk_annot :t:
-  Smt (DeclareConst 4516%Z Ty_Bool) Mk_annot :t:
-  WriteMem (RegVal_Base (Val_Symbolic 4516%Z)) (RegVal_Base (Val_Enum ((Mk_enum_id 6%nat), Mk_enum_ctor 0%nat))) (RegVal_Base (Val_Symbolic 4515%Z)) (RegVal_Base (Val_Symbolic 77%Z)) 8%N None Mk_annot :t:
-  Smt (DeclareConst 4517%Z (Ty_BitVec 64%N)) Mk_annot :t:
-  ReadReg "_PC" [] (RegVal_Base (Val_Symbolic 4517%Z)) Mk_annot :t:
-  Smt (DefineConst 4518%Z (Manyop (Bvmanyarith Bvadd) [Val (Val_Symbolic 4517%Z) Mk_annot; Val (Val_Bits (BV 64%N 0x4%Z)) Mk_annot] Mk_annot)) Mk_annot :t:
-  WriteReg "_PC" [] (RegVal_Base (Val_Symbolic 4518%Z)) Mk_annot :t:
+  ReadReg "SP_EL2" [] (RegVal_Base (Val_Symbolic 26%Z)) Mk_annot :t:
+  Smt (DefineConst 36%Z (Manyop (Bvmanyarith Bvadd) [Val (Val_Symbolic 26%Z) Mk_annot; Val (Val_Bits (BV 64%N 0x30%Z)) Mk_annot] Mk_annot)) Mk_annot :t:
+  Smt (DeclareConst 37%Z (Ty_BitVec 64%N)) Mk_annot :t:
+  ReadReg "R20" [] (RegVal_Base (Val_Symbolic 37%Z)) Mk_annot :t:
+  Smt (DefineConst 38%Z (Val (Val_Symbolic 37%Z) Mk_annot)) Mk_annot :t:
+  Smt (DeclareConst 39%Z (Ty_BitVec 64%N)) Mk_annot :t:
+  ReadReg "R19" [] (RegVal_Base (Val_Symbolic 39%Z)) Mk_annot :t:
+  Smt (DefineConst 40%Z (Val (Val_Symbolic 39%Z) Mk_annot)) Mk_annot :t:
+  Smt (DefineConst 41%Z (Manyop (Bvmanyarith Bvadd) [Val (Val_Symbolic 36%Z) Mk_annot; Val (Val_Bits (BV 64%N 0x0%Z)) Mk_annot] Mk_annot)) Mk_annot :t:
+  Smt (DefineConst 46%Z (Binop (Eq) (Val (Val_Symbolic 41%Z) Mk_annot) (Manyop (Bvmanyarith Bvand) [Val (Val_Symbolic 41%Z) Mk_annot; Val (Val_Bits (BV 64%N 0xfffffffffffffff8%Z)) Mk_annot] Mk_annot) Mk_annot)) Mk_annot :t:
+  ReadReg "PSTATE" [Field "D"] (RegVal_Struct [("D", RegVal_Base (Val_Symbolic 3%Z))]) Mk_annot :t:
+  Smt (DefineConst 1220%Z (Val (Val_Symbolic 41%Z) Mk_annot)) Mk_annot :t:
+  Smt (DeclareConst 1221%Z (Ty_BitVec 64%N)) Mk_annot :t:
+  ReadReg "MPIDR_EL1" [] (RegVal_Base (Val_Symbolic 1221%Z)) Mk_annot :t:
+  Smt (DefineConst 1375%Z (Manyop Concat [Val (Val_Bits (BV 4%N 0x0%Z)) Mk_annot; Unop (Extract 51%N 0%N) (Val (Val_Symbolic 41%Z) Mk_annot) Mk_annot] Mk_annot)) Mk_annot :t:
+  Smt (DefineConst 1376%Z (Unop (ZeroExtend 8%N) (Val (Val_Symbolic 1375%Z) Mk_annot) Mk_annot)) Mk_annot :t:
+  Smt (DeclareConst 1377%Z Ty_Bool) Mk_annot :t:
+  WriteMem (RegVal_Base (Val_Symbolic 1377%Z)) (RegVal_Poison) (RegVal_Base (Val_Symbolic 1376%Z)) (RegVal_Base (Val_Symbolic 38%Z)) 8%N None Mk_annot :t:
+  Smt (DefineConst 1378%Z (Manyop (Bvmanyarith Bvadd) [Val (Val_Symbolic 36%Z) Mk_annot; Val (Val_Bits (BV 64%N 0x8%Z)) Mk_annot] Mk_annot)) Mk_annot :t:
+  Smt (DefineConst 1383%Z (Binop (Eq) (Val (Val_Symbolic 1378%Z) Mk_annot) (Manyop (Bvmanyarith Bvand) [Val (Val_Symbolic 1378%Z) Mk_annot; Val (Val_Bits (BV 64%N 0xfffffffffffffff8%Z)) Mk_annot] Mk_annot) Mk_annot)) Mk_annot :t:
+  Smt (DefineConst 2557%Z (Val (Val_Symbolic 1378%Z) Mk_annot)) Mk_annot :t:
+  Smt (DefineConst 2711%Z (Manyop Concat [Val (Val_Bits (BV 4%N 0x0%Z)) Mk_annot; Unop (Extract 51%N 0%N) (Val (Val_Symbolic 1378%Z) Mk_annot) Mk_annot] Mk_annot)) Mk_annot :t:
+  Smt (DefineConst 2712%Z (Unop (ZeroExtend 8%N) (Val (Val_Symbolic 2711%Z) Mk_annot) Mk_annot)) Mk_annot :t:
+  Smt (DeclareConst 2713%Z Ty_Bool) Mk_annot :t:
+  WriteMem (RegVal_Base (Val_Symbolic 2713%Z)) (RegVal_Poison) (RegVal_Base (Val_Symbolic 2712%Z)) (RegVal_Base (Val_Symbolic 40%Z)) 8%N None Mk_annot :t:
+  Smt (DeclareConst 2714%Z (Ty_BitVec 64%N)) Mk_annot :t:
+  ReadReg "_PC" [] (RegVal_Base (Val_Symbolic 2714%Z)) Mk_annot :t:
+  Smt (DefineConst 2715%Z (Manyop (Bvmanyarith Bvadd) [Val (Val_Symbolic 2714%Z) Mk_annot; Val (Val_Bits (BV 64%N 0x4%Z)) Mk_annot] Mk_annot)) Mk_annot :t:
+  WriteReg "_PC" [] (RegVal_Base (Val_Symbolic 2715%Z)) Mk_annot :t:
   tnil
 .
