instructions/hello/a1c.v
@@ -10,24 +10,24 @@ Definition a1c : isla_trace :=
   AssumeReg "PSTATE" [Field "EL"] (RegVal_Base (Val_Bits (BV 2%N 0x2%Z))) Mk_annot :t:
   AssumeReg "PSTATE" [Field "nRW"] (RegVal_Base (Val_Bits (BV 1%N 0x0%Z))) Mk_annot :t:
   AssumeReg "SCR_EL3" [] (RegVal_Base (Val_Bits (BV 32%N 0x501%Z))) Mk_annot :t:
-  Smt (DeclareConst 36%Z (Ty_BitVec 64%N)) Mk_annot :t:
-  ReadReg "R0" [] (RegVal_Base (Val_Symbolic 36%Z)) Mk_annot :t:
-  Smt (DefineConst 39%Z (Binop (Eq) (Binop (Eq) (Unop (Extract 31%N 0%N) (Val (Val_Symbolic 36%Z) Mk_annot) Mk_annot) (Val (Val_Bits (BV 32%N 0x0%Z)) Mk_annot) Mk_annot) (Val (Val_Bool false) Mk_annot) Mk_annot)) Mk_annot :t:
+  Smt (DeclareConst 26%Z (Ty_BitVec 64%N)) Mk_annot :t:
+  ReadReg "R0" [] (RegVal_Base (Val_Symbolic 26%Z)) Mk_annot :t:
+  Smt (DefineConst 29%Z (Binop (Eq) (Binop (Eq) (Unop (Extract 31%N 0%N) (Val (Val_Symbolic 26%Z) Mk_annot) Mk_annot) (Val (Val_Bits (BV 32%N 0x0%Z)) Mk_annot) Mk_annot) (Val (Val_Bool false) Mk_annot) Mk_annot)) Mk_annot :t:
   tcases [
-    Smt (Assert (Val (Val_Symbolic 39%Z) Mk_annot)) Mk_annot :t:
-    Smt (DeclareConst 40%Z (Ty_BitVec 64%N)) Mk_annot :t:
-    ReadReg "_PC" [] (RegVal_Base (Val_Symbolic 40%Z)) Mk_annot :t:
-    Smt (DefineConst 41%Z (Manyop (Bvmanyarith Bvadd) [Val (Val_Symbolic 40%Z) Mk_annot; Val (Val_Bits (BV 64%N 0xfffffffffffffff8%Z)) Mk_annot] Mk_annot)) Mk_annot :t:
-    Smt (DefineConst 53%Z (Val (Val_Symbolic 41%Z) Mk_annot)) Mk_annot :t:
-    BranchAddress (RegVal_Base (Val_Symbolic 53%Z)) Mk_annot :t:
-    Smt (DefineConst 54%Z (Val (Val_Symbolic 41%Z) Mk_annot)) Mk_annot :t:
-    WriteReg "_PC" [] (RegVal_Base (Val_Symbolic 54%Z)) Mk_annot :t:
+    Smt (Assert (Val (Val_Symbolic 29%Z) Mk_annot)) Mk_annot :t:
+    Smt (DeclareConst 30%Z (Ty_BitVec 64%N)) Mk_annot :t:
+    ReadReg "_PC" [] (RegVal_Base (Val_Symbolic 30%Z)) Mk_annot :t:
+    Smt (DefineConst 31%Z (Manyop (Bvmanyarith Bvadd) [Val (Val_Symbolic 30%Z) Mk_annot; Val (Val_Bits (BV 64%N 0xfffffffffffffff8%Z)) Mk_annot] Mk_annot)) Mk_annot :t:
+    Smt (DefineConst 32%Z (Val (Val_Symbolic 31%Z) Mk_annot)) Mk_annot :t:
+    BranchAddress (RegVal_Base (Val_Symbolic 32%Z)) Mk_annot :t:
+    Smt (DefineConst 33%Z (Val (Val_Symbolic 31%Z) Mk_annot)) Mk_annot :t:
+    WriteReg "_PC" [] (RegVal_Base (Val_Symbolic 33%Z)) Mk_annot :t:
     tnil;
-    Smt (Assert (Unop (Not) (Val (Val_Symbolic 39%Z) Mk_annot) Mk_annot)) Mk_annot :t:
-    Smt (DeclareConst 40%Z (Ty_BitVec 64%N)) Mk_annot :t:
-    ReadReg "_PC" [] (RegVal_Base (Val_Symbolic 40%Z)) Mk_annot :t:
-    Smt (DefineConst 41%Z (Manyop (Bvmanyarith Bvadd) [Val (Val_Symbolic 40%Z) Mk_annot; Val (Val_Bits (BV 64%N 0x4%Z)) Mk_annot] Mk_annot)) Mk_annot :t:
-    WriteReg "_PC" [] (RegVal_Base (Val_Symbolic 41%Z)) Mk_annot :t:
+    Smt (Assert (Unop (Not) (Val (Val_Symbolic 29%Z) Mk_annot) Mk_annot)) Mk_annot :t:
+    Smt (DeclareConst 51%Z (Ty_BitVec 64%N)) Mk_annot :t:
+    ReadReg "_PC" [] (RegVal_Base (Val_Symbolic 51%Z)) Mk_annot :t:
+    Smt (DefineConst 52%Z (Manyop (Bvmanyarith Bvadd) [Val (Val_Symbolic 51%Z) Mk_annot; Val (Val_Bits (BV 64%N 0x4%Z)) Mk_annot] Mk_annot)) Mk_annot :t:
+    WriteReg "_PC" [] (RegVal_Base (Val_Symbolic 52%Z)) Mk_annot :t:
     tnil
   ]
 .
