instructions/riscv64_test/a10.v
@@ -5,19 +5,19 @@ Definition a10 : isla_trace :=
   Assume (AExp_Binop (Eq) (AExp_Unop (Extract 1%N 1%N) (AExp_Val (AVal_Var "PC" []) Mk_annot) Mk_annot) (AExp_Val (AVal_Bits (BV 1%N 0x0%Z)) Mk_annot) Mk_annot) Mk_annot :t:
   ReadReg "PC" [] (RegVal_Base (Val_Symbolic 0%Z)) Mk_annot :t:
   Smt (DefineConst 1%Z (Manyop (Bvmanyarith Bvadd) [Val (Val_Symbolic 0%Z) Mk_annot; Val (Val_Bits (BV 64%N 0x4%Z)) Mk_annot] Mk_annot)) Mk_annot :t:
-  Smt (DeclareConst 13%Z (Ty_BitVec 64%N)) Mk_annot :t:
-  ReadReg "x10" [] (RegVal_Base (Val_Symbolic 13%Z)) Mk_annot :t:
-  Smt (DeclareConst 14%Z (Ty_BitVec 64%N)) Mk_annot :t:
-  ReadReg "x11" [] (RegVal_Base (Val_Symbolic 14%Z)) Mk_annot :t:
-  Smt (DefineConst 15%Z (Binop (Eq) (Val (Val_Symbolic 13%Z) Mk_annot) (Val (Val_Symbolic 14%Z) Mk_annot) Mk_annot)) Mk_annot :t:
-  Smt (DefineConst 16%Z (Manyop (Bvmanyarith Bvadd) [Val (Val_Symbolic 0%Z) Mk_annot; Val (Val_Bits (BV 64%N 0x8%Z)) Mk_annot] Mk_annot)) Mk_annot :t:
+  Smt (DeclareConst 2%Z (Ty_BitVec 64%N)) Mk_annot :t:
+  ReadReg "x10" [] (RegVal_Base (Val_Symbolic 2%Z)) Mk_annot :t:
+  Smt (DeclareConst 3%Z (Ty_BitVec 64%N)) Mk_annot :t:
+  ReadReg "x11" [] (RegVal_Base (Val_Symbolic 3%Z)) Mk_annot :t:
+  Smt (DefineConst 4%Z (Binop (Eq) (Val (Val_Symbolic 2%Z) Mk_annot) (Val (Val_Symbolic 3%Z) Mk_annot) Mk_annot)) Mk_annot :t:
+  Smt (DefineConst 5%Z (Manyop (Bvmanyarith Bvadd) [Val (Val_Symbolic 0%Z) Mk_annot; Val (Val_Bits (BV 64%N 0x8%Z)) Mk_annot] Mk_annot)) Mk_annot :t:
   tcases [
-    Smt (Assert (Val (Val_Symbolic 15%Z) Mk_annot)) Mk_annot :t:
-    Smt (DefineConst 17%Z (Unop (Extract 0%N 0%N) (Binop ((Bvarith Bvlshr)) (Val (Val_Symbolic 16%Z) Mk_annot) (Val (Val_Bits (BV 64%N 0x1%Z)) Mk_annot) Mk_annot) Mk_annot)) Mk_annot :t:
-    BranchAddress (RegVal_Base (Val_Symbolic 16%Z)) Mk_annot :t:
-    WriteReg "PC" [] (RegVal_Base (Val_Symbolic 16%Z)) Mk_annot :t:
+    Smt (Assert (Val (Val_Symbolic 4%Z) Mk_annot)) Mk_annot :t:
+    Smt (DefineConst 6%Z (Unop (Extract 0%N 0%N) (Binop ((Bvarith Bvlshr)) (Val (Val_Symbolic 5%Z) Mk_annot) (Val (Val_Bits (BV 64%N 0x1%Z)) Mk_annot) Mk_annot) Mk_annot)) Mk_annot :t:
+    BranchAddress (RegVal_Base (Val_Symbolic 5%Z)) Mk_annot :t:
+    WriteReg "PC" [] (RegVal_Base (Val_Symbolic 5%Z)) Mk_annot :t:
     tnil;
-    Smt (Assert (Unop (Not) (Val (Val_Symbolic 15%Z) Mk_annot) Mk_annot)) Mk_annot :t:
+    Smt (Assert (Unop (Not) (Val (Val_Symbolic 4%Z) Mk_annot) Mk_annot)) Mk_annot :t:
     WriteReg "PC" [] (RegVal_Base (Val_Symbolic 1%Z)) Mk_annot :t:
     tnil
   ]
