instructions/uart/a80184.v
@@ -10,26 +10,27 @@ Definition a80184 : isla_trace :=
   AssumeReg "EDSCR" [] (RegVal_Base (Val_Bits (BV 32%N 0x0%Z))) Mk_annot :t:
   AssumeReg "OSDLR_EL1" [] (RegVal_Base (Val_Bits (BV 32%N 0x0%Z))) Mk_annot :t:
   AssumeReg "OSLSR_EL1" [] (RegVal_Base (Val_Bits (BV 32%N 0x0%Z))) Mk_annot :t:
-  Smt (DeclareConst 6%Z (Ty_BitVec 1%N)) Mk_annot :t:
+  Smt (DeclareConst 3%Z (Ty_BitVec 1%N)) Mk_annot :t:
   AssumeReg "PSTATE" [Field "EL"] (RegVal_Base (Val_Bits (BV 2%N 0x2%Z))) Mk_annot :t:
   AssumeReg "PSTATE" [Field "nRW"] (RegVal_Base (Val_Bits (BV 1%N 0x0%Z))) Mk_annot :t:
   AssumeReg "SCR_EL3" [] (RegVal_Base (Val_Bits (BV 32%N 0x501%Z))) Mk_annot :t:
   AssumeReg "SCTLR_EL2" [] (RegVal_Base (Val_Bits (BV 64%N 0x4000002%Z))) Mk_annot :t:
-  Smt (DeclareConst 29%Z (Ty_BitVec 64%N)) Mk_annot :t:
+  Smt (DeclareConst 26%Z (Ty_BitVec 64%N)) Mk_annot :t:
   Assume (AExp_Binop (Eq) (AExp_Manyop (Bvmanyarith Bvand) [AExp_Val (AVal_Var "R2" []) Mk_annot; AExp_Val (AVal_Bits (BV 64%N 0xfff0000000000003%Z)) Mk_annot] Mk_annot) (AExp_Val (AVal_Bits (BV 64%N 0x0%Z)) Mk_annot) Mk_annot) Mk_annot :t:
-  ReadReg "R2" [] (RegVal_Base (Val_Symbolic 29%Z)) Mk_annot :t:
-  Smt (DefineConst 118%Z (Manyop (Bvmanyarith Bvadd) [Val (Val_Symbolic 29%Z) Mk_annot; Val (Val_Bits (BV 64%N 0x0%Z)) Mk_annot] Mk_annot)) Mk_annot :t:
-  Smt (DefineConst 122%Z (Binop (Eq) (Val (Val_Symbolic 118%Z) Mk_annot) (Manyop (Bvmanyarith Bvand) [Val (Val_Symbolic 118%Z) Mk_annot; Val (Val_Bits (BV 64%N 0xfffffffffffffffc%Z)) Mk_annot] Mk_annot) Mk_annot)) Mk_annot :t:
-  ReadReg "PSTATE" [Field "D"] (RegVal_Struct [("D", RegVal_Base (Val_Symbolic 6%Z))]) Mk_annot :t:
-  Smt (DeclareConst 2317%Z (Ty_BitVec 56%N)) Mk_annot :t:
-  Smt (DefineConst 2326%Z (Unop (ZeroExtend 8%N) (Manyop Concat [Val (Val_Bits (BV 4%N 0x0%Z)) Mk_annot; Unop (Extract 51%N 0%N) (Val (Val_Symbolic 118%Z) Mk_annot) Mk_annot] Mk_annot) Mk_annot)) Mk_annot :t:
-  Smt (DeclareConst 2327%Z (Ty_BitVec 32%N)) Mk_annot :t:
-  ReadMem (RegVal_Base (Val_Symbolic 2327%Z)) (RegVal_Base (Val_Enum ((Mk_enum_id 6%nat), Mk_enum_ctor 0%nat))) (RegVal_Base (Val_Symbolic 2326%Z)) 4%N None Mk_annot :t:
-  Smt (DefineConst 2331%Z (Manyop Concat [Val (Val_Bits (BV 32%N 0x0%Z)) Mk_annot; Val (Val_Symbolic 2327%Z) Mk_annot] Mk_annot)) Mk_annot :t:
-  WriteReg "R1" [] (RegVal_Base (Val_Symbolic 2331%Z)) Mk_annot :t:
-  Smt (DeclareConst 2332%Z (Ty_BitVec 64%N)) Mk_annot :t:
-  ReadReg "_PC" [] (RegVal_Base (Val_Symbolic 2332%Z)) Mk_annot :t:
-  Smt (DefineConst 2333%Z (Manyop (Bvmanyarith Bvadd) [Val (Val_Symbolic 2332%Z) Mk_annot; Val (Val_Bits (BV 64%N 0x4%Z)) Mk_annot] Mk_annot)) Mk_annot :t:
-  WriteReg "_PC" [] (RegVal_Base (Val_Symbolic 2333%Z)) Mk_annot :t:
+  ReadReg "R2" [] (RegVal_Base (Val_Symbolic 26%Z)) Mk_annot :t:
+  Smt (DefineConst 65%Z (Manyop (Bvmanyarith Bvadd) [Val (Val_Symbolic 26%Z) Mk_annot; Val (Val_Bits (BV 64%N 0x0%Z)) Mk_annot] Mk_annot)) Mk_annot :t:
+  Smt (DefineConst 69%Z (Binop (Eq) (Val (Val_Symbolic 65%Z) Mk_annot) (Manyop (Bvmanyarith Bvand) [Val (Val_Symbolic 65%Z) Mk_annot; Val (Val_Bits (BV 64%N 0xfffffffffffffffc%Z)) Mk_annot] Mk_annot) Mk_annot)) Mk_annot :t:
+  ReadReg "PSTATE" [Field "D"] (RegVal_Struct [("D", RegVal_Base (Val_Symbolic 3%Z))]) Mk_annot :t:
+  Smt (DefineConst 1244%Z (Val (Val_Symbolic 65%Z) Mk_annot)) Mk_annot :t:
+  Smt (DefineConst 1392%Z (Manyop Concat [Val (Val_Bits (BV 4%N 0x0%Z)) Mk_annot; Unop (Extract 51%N 0%N) (Val (Val_Symbolic 65%Z) Mk_annot) Mk_annot] Mk_annot)) Mk_annot :t:
+  Smt (DefineConst 1393%Z (Unop (ZeroExtend 8%N) (Val (Val_Symbolic 1392%Z) Mk_annot) Mk_annot)) Mk_annot :t:
+  Smt (DeclareConst 1394%Z (Ty_BitVec 32%N)) Mk_annot :t:
+  ReadMem (RegVal_Base (Val_Symbolic 1394%Z)) (RegVal_Poison) (RegVal_Base (Val_Symbolic 1393%Z)) 4%N None Mk_annot :t:
+  Smt (DefineConst 1398%Z (Manyop Concat [Val (Val_Bits (BV 32%N 0x0%Z)) Mk_annot; Val (Val_Symbolic 1394%Z) Mk_annot] Mk_annot)) Mk_annot :t:
+  WriteReg "R1" [] (RegVal_Base (Val_Symbolic 1398%Z)) Mk_annot :t:
+  Smt (DeclareConst 1399%Z (Ty_BitVec 64%N)) Mk_annot :t:
+  ReadReg "_PC" [] (RegVal_Base (Val_Symbolic 1399%Z)) Mk_annot :t:
+  Smt (DefineConst 1400%Z (Manyop (Bvmanyarith Bvadd) [Val (Val_Symbolic 1399%Z) Mk_annot; Val (Val_Bits (BV 64%N 0x4%Z)) Mk_annot] Mk_annot)) Mk_annot :t:
+  WriteReg "_PC" [] (RegVal_Base (Val_Symbolic 1400%Z)) Mk_annot :t:
   tnil
 .
