instructions/uart/a80190.v
@@ -1,13 +1,13 @@
 From isla Require Import opsem.
 
 Definition a80190 : isla_trace :=
-  Smt (DeclareConst 46%Z (Ty_BitVec 64%N)) Mk_annot :t:
-  ReadReg "R1" [] (RegVal_Base (Val_Symbolic 46%Z)) Mk_annot :t:
-  Smt (DefineConst 49%Z (Manyop (Bvmanyarith Bvor) [Manyop (Bvmanyarith Bvand) [Val (Val_Symbolic 46%Z) Mk_annot; Val (Val_Bits (BV 64%N 0xffffffff0000ffff%Z)) Mk_annot] Mk_annot; Val (Val_Bits (BV 64%N 0x3f210000%Z)) Mk_annot] Mk_annot)) Mk_annot :t:
-  WriteReg "R1" [] (RegVal_Base (Val_Symbolic 49%Z)) Mk_annot :t:
-  Smt (DeclareConst 50%Z (Ty_BitVec 64%N)) Mk_annot :t:
-  ReadReg "_PC" [] (RegVal_Base (Val_Symbolic 50%Z)) Mk_annot :t:
-  Smt (DefineConst 51%Z (Manyop (Bvmanyarith Bvadd) [Val (Val_Symbolic 50%Z) Mk_annot; Val (Val_Bits (BV 64%N 0x4%Z)) Mk_annot] Mk_annot)) Mk_annot :t:
-  WriteReg "_PC" [] (RegVal_Base (Val_Symbolic 51%Z)) Mk_annot :t:
+  Smt (DeclareConst 32%Z (Ty_BitVec 64%N)) Mk_annot :t:
+  ReadReg "R1" [] (RegVal_Base (Val_Symbolic 32%Z)) Mk_annot :t:
+  Smt (DefineConst 35%Z (Manyop (Bvmanyarith Bvor) [Manyop (Bvmanyarith Bvand) [Val (Val_Symbolic 32%Z) Mk_annot; Val (Val_Bits (BV 64%N 0xffffffff0000ffff%Z)) Mk_annot] Mk_annot; Val (Val_Bits (BV 64%N 0x3f210000%Z)) Mk_annot] Mk_annot)) Mk_annot :t:
+  WriteReg "R1" [] (RegVal_Base (Val_Symbolic 35%Z)) Mk_annot :t:
+  Smt (DeclareConst 36%Z (Ty_BitVec 64%N)) Mk_annot :t:
+  ReadReg "_PC" [] (RegVal_Base (Val_Symbolic 36%Z)) Mk_annot :t:
+  Smt (DefineConst 37%Z (Manyop (Bvmanyarith Bvadd) [Val (Val_Symbolic 36%Z) Mk_annot; Val (Val_Bits (BV 64%N 0x4%Z)) Mk_annot] Mk_annot)) Mk_annot :t:
+  WriteReg "_PC" [] (RegVal_Base (Val_Symbolic 37%Z)) Mk_annot :t:
   tnil
 .
