pkvm_handler/a18270.v
@@ -1,9 +1,9 @@
 From isla Require Import opsem.
 
 Definition a18270 : isla_trace :=
-  Smt (DeclareConst 68%Z (Ty_BitVec 64%N)) Mk_annot :t:
-  ReadReg "_PC" [] (RegVal_Base (Val_Symbolic 68%Z)) Mk_annot :t:
-  Smt (DefineConst 69%Z (Manyop (Bvmanyarith Bvadd) [Val (Val_Symbolic 68%Z) Mk_annot; Val (Val_Bits (BV 64%N 0x4%Z)) Mk_annot] Mk_annot)) Mk_annot :t:
-  WriteReg "_PC" [] (RegVal_Base (Val_Symbolic 69%Z)) Mk_annot :t:
+  Smt (DeclareConst 46%Z (Ty_BitVec 64%N)) Mk_annot :t:
+  ReadReg "_PC" [] (RegVal_Base (Val_Symbolic 46%Z)) Mk_annot :t:
+  Smt (DefineConst 47%Z (Manyop (Bvmanyarith Bvadd) [Val (Val_Symbolic 46%Z) Mk_annot; Val (Val_Bits (BV 64%N 0x4%Z)) Mk_annot] Mk_annot)) Mk_annot :t:
+  WriteReg "_PC" [] (RegVal_Base (Val_Symbolic 47%Z)) Mk_annot :t:
   tnil
 .
