update_isla_lang.sh
@@ -4,11 +4,10 @@
 # the repository. Note that the script is self-modifying: it will change the
 # old hash into the new one, and erase the new hash again.
 
-OLD_HASH=14541f64fc25f98ce77be070d1fa3a8eb08207dc
+OLD_HASH=4ee3daa3a9f04b2d6a55dd94026ff5f9d79db5fc
 NEW_HASH=
 
 sed -i "s/${OLD_HASH}/${NEW_HASH}/g" README.md .gitlab-ci.yml .github/workflows/ci.yml update_isla_lang.sh Makefile
 sed -i "s/^NEW_HASH=.*/NEW_HASH=/g" update_isla_lang.sh
 
-opam pin remove -y isla-lang
-opam pin add -n -y isla-lang "git+https://github.com/rems-project/isla-lang.git#${NEW_HASH}"
+make builddep
